\begin{exercise}{
    Let $C$ and $A$ be complete lattices and let $(\alpha, C, A, \gamma)$ be a Galois connection. Prove the following properties:
    \begin{enumerate}[(1)]
        \item for any $c_1, c_2 \in C, \gamma(\alpha(c_1 \vee_C c_2)) = \gamma(\alpha(\gamma(\alpha(c_1)) \vee_C \gamma(\alpha(c_2))))$
        \item for all $S \subseteq A, \gamma(\wedge_A S) = \wedge_C \left\{\gamma(a) \in C \mid a \in S \right\}$
        \item $\gamma$ is injective if and only if $\alpha \circ \gamma = \id$ if and only if $\alpha$ is surjective.
    \end{enumerate}
}
    \begin{enumerate}[(1)]
        \item We prove the two directions:
        \begin{itemize}
            \item $(\leq)$:
            \begin{gather*}
                c_i \leq \gamma(\alpha(c_i)) \leq \gamma(\alpha(c_1)) \vee_C \gamma(\alpha(c_2)) \quad\quad \forall i \in \left\{ 1, 2 \right\} \\
                \implies c_1 \vee_C c_2 \leq \gamma(\alpha(c_1)) \vee_C \gamma(\alpha(c_2)) \\
                \implies \gamma(\alpha(c_1 \vee_C c_2)) \leq \gamma(\alpha(\gamma(\alpha(c_1)) \vee_C \gamma(\alpha(c_2))))
            \end{gather*}
            \item $(\geq)$:
            \begin{gather*}
                c_i \leq c_1 \vee_C c_2 \quad\quad \forall i \in \left\{ 1, 2 \right\} \\
                \implies \gamma(\alpha(c_i)) \leq \gamma(\alpha(c_1 \vee_C c_2)) \quad\quad \forall i \in \left\{ 1, 2 \right\} \\
                \implies \gamma(\alpha(c_1)) \vee_C \gamma(\alpha(c_2)) \leq \gamma(\alpha(c_1 \vee_C c_2)) \\
                \implies \alpha(\gamma(\alpha(c_1)) \vee_C \gamma(\alpha(c_2))) \leq \alpha(c_1 \vee_C c_2) \\
                \implies \gamma(\alpha(\gamma(\alpha(c_1)) \vee_C \gamma(\alpha(c_2)))) \leq \gamma(\alpha(c_1 \vee_C c_2))
            \end{gather*}
        \end{itemize}
        \item We prove the two directions:
        \begin{itemize}
            \item $(\leq)$:
            \begin{gather*}
                \wedge_A S \leq a \quad \forall a \in S \\
                \implies \gamma(\wedge_A S) \leq \gamma(a) \quad \forall a \in S \\
                \implies \gamma(\wedge_A S) \leq \wedge_C \left\{\gamma(a) \in C \mid a \in S\right\}
            \end{gather*}
            \item $(\geq)$:
            \begin{gather*}
                \wedge_C \left\{\gamma(a) \in C \mid a \in S\right\} \leq \gamma(a) \quad \forall a \in S \\
                \implies \alpha(\wedge_C \left\{\gamma(a) \in C \mid a \in S\right\}) \leq a \quad \forall a \in S \\
                \implies \alpha(\wedge_C \left\{\gamma(a) \in C \mid a \in S\right\}) \leq \wedge_A S \\
                \implies \wedge_C \left\{\gamma(a) \in C \mid a \in S\right\} \leq \gamma(\wedge_A S)
            \end{gather*}
        \end{itemize}
        \item This is the definition of a Galois Insertion. We prove this by proving the following:
        \begin{itemize}
            \item $\gamma$ is injective $\implies \alpha \circ \gamma = \id$
            \begin{gather*}
                \gamma(a) \leq \gamma(\alpha(\gamma(a))) \\
                \alpha(\gamma(a)) \leq a
                \implies \gamma(\alpha(\gamma(a))) \leq \gamma(a) \\
                \implies \gamma(a) = \gamma(\alpha(\gamma(a))) \\
                \iff a = \alpha(\gamma(a))
            \end{gather*}
            \item $\alpha \circ \gamma = \id \implies \alpha$ is surjective
            \begin{gather*}
                \forall a \in A.\ \alpha(\gamma(a)) = a \\
                \implies \forall a \in A.\ \exists c = \gamma(a) \in C.\ \alpha(c) = a \\
                \implies \alpha \text{ is surjective}
            \end{gather*}
            \item $\alpha$ surjective $\implies \gamma$ injective
            \begin{gather*}
                \alpha(\gamma(\alpha(c))) \leq \alpha(c) \\
                c \leq \gamma(\alpha(c))
                \implies \alpha(c) \leq \alpha(\gamma(\alpha(c))) \\
                \implies \alpha(c) = \alpha(\gamma(\alpha(c))) \\
                \alpha \text{ surjective } \implies \forall a \in A.\ \exists c \in C.\ \alpha(c) = a \\
                \forall a_1, a_2 \in A.\ \gamma(a_1) = \gamma(a_2) \implies \\
                a_1 = \alpha(c_1) = \alpha(\gamma(\alpha(c_1))) = \alpha(\gamma(a_1)) = \alpha(\gamma(a_2)) = \alpha(\gamma(\alpha(c_2))) = \alpha(c_2) = a_2
            \end{gather*}
        \end{itemize}
    \end{enumerate}
\end{exercise}
