\begin{exercise}{
    Let $C$ and $A$ be complete lattices, $(\alpha, C, A, \gamma)$ be a Galois insertion, $f: C \to C$ be a monotone function. Prove that $\gamma(\lfp(\alpha \circ f \circ \gamma)) = \lfp(\gamma \circ \alpha \circ f)$
}
    We prove the two directions:
    \begin{itemize}
        \item $\leq$
        \begin{gather*}
            \begin{aligned}
                (\alpha \circ f)(\lfp(\gamma \circ \alpha \circ f))
                &= (\alpha \circ f \circ \gamma \circ \alpha \circ f)(\lfp(\gamma \circ \alpha \circ f)) \\
                &= (\alpha \circ f \circ \gamma)((\alpha \circ f)(\lfp(\gamma \circ \alpha \circ f)))
            \end{aligned} \\
            \implies \lfp(\alpha \circ f \circ \gamma) \leq (\alpha \circ f)(\lfp(\gamma \circ \alpha \circ f)) \\
            \implies \gamma(\lfp(\alpha \circ f \circ \gamma)) \leq (\gamma \circ \alpha \circ f)(\lfp(\gamma \circ \alpha \circ f)) = \lfp(\gamma \circ \alpha \circ f)
        \end{gather*}
        \item $\geq$
        \begin{gather*}
            \begin{aligned}
                \gamma(\lfp(\alpha \circ f \circ \gamma))
                &= (\gamma \circ \alpha \circ f \circ \gamma) (\lfp(\alpha \circ f \circ \gamma)) \\
                &= (\gamma \circ \alpha \circ f)(\gamma(\lfp(\alpha \circ f \circ \gamma)))
            \end{aligned} \\
            \implies \lfp(\gamma \circ \alpha \circ f) \leq \gamma(\lfp(\alpha \circ f \circ \gamma))
        \end{gather*}
    \end{itemize}
\end{exercise}
